Parse and type-check function tag

src/Ast/Ast.dfy
@@ -12,7 +12,7 @@ module Ast {
     provides Procedure.Name, Procedure.Parameters, Procedure.Pre, Procedure.Post, Procedure.Body
     reveals Procedure.SignatureWellFormed, Procedure.WellFormedHeader
     reveals Function, FParameter, FunctionDefinition
-    provides Function.Name, Function.Parameters, Function.ResultType, Function.Definition, FParameter.injective
+    provides Function.Name, Function.Parameters, Function.ResultType, Function.Tag, Function.Definition, FParameter.injective
     reveals Function.SignatureWellFormed, Function.WellFormed, FParameter.WellFormed, FunctionDefinition.WellFormed
     reveals Tagger, Tagger.Name, Tagger.ForType, Tagger.WellFormed
     provides Variable.name, Variable.typ
@@ -148,14 +148,16 @@ module Ast {
     const Name: string
     const Parameters: seq<FParameter>
     const ResultType: Type
+    const Tag: Option<Tagger>
     var Definition: Option<FunctionDefinition>
 
-    constructor (name: string, parameters: seq<FParameter>, resultType: Type)
-      ensures Name == name && Parameters == parameters && ResultType == resultType && Definition == None
+    constructor (name: string, parameters: seq<FParameter>, resultType: Type, maybeTag: Option<Tagger>)
+      ensures Name == name && Parameters == parameters && ResultType == resultType && Tag == maybeTag && Definition == None
     {
       Name := name;
       Parameters := parameters;
       ResultType := resultType;
+      Tag := maybeTag;
       Definition := None;
     }
 
@@ -167,6 +169,8 @@ module Ast {
       && (forall i :: 0 <= i < |Parameters| ==> Parameters[i].name == func.parameters[i].name)
       && (forall i :: 0 <= i < |Parameters| ==> Parameters[i].injective == func.parameters[i].injective)
       && (forall i :: 0 <= i < |Parameters| ==> Parameters[i].WellFormed())
+      && (if func.tag == None then Tag == None else Tag.Some? && Tag.value.Name == func.tag.value)
+      && (Tag.Some? ==> Tag.value.ForType == ResultType)
     }
 
     predicate WellFormed()
@@ -175,6 +179,7 @@ module Ast {
       && (forall i :: 0 <= i < |Parameters| ==> Parameters[i].WellFormed())
       && (forall i, j :: 0 <= i < j < |Parameters| ==> Parameters[i].name != Parameters[j].name)
       && (Definition == None || Definition.value.WellFormed())
+      && (Tag.Some? ==> Tag.value.ForType == ResultType)
     }
   }
 
